Refactoring word theory

opentheory/theories/all.ml
@@ -121,6 +121,7 @@ loads "opentheory/theories/gfp/gfp.ml";;
 (* Parametric theory of words.                                               *)
 (* ------------------------------------------------------------------------- *)
 
+(***
 loads "opentheory/theories/word/word.ml";;
 
 (* ------------------------------------------------------------------------- *)
@@ -184,3 +185,4 @@ loads "opentheory/theories/h/h.ml";;
 (* Requires MiniSat to be hooked up to HOL Light
 loads "opentheory/theories/map-reduce-bit3x3/map-reduce-bit3x3.ml";;
 *)
+***)
